<rdf:RDF xml:base="https://dmaus.name/ns/vrsl"
         xmlns:rdf="http://www.w3.org/1999/02/22-rdf-syntax-ns#"
         xmlns:rdfs="http://www.w3.org/2000/01/rdf-schema#"
         xmlns:sh="http://www.w3.org/ns/shacl#">

  <!-- Formal description of the VRSL ontology -->
  <rdfs:Class rdf:about="#ValidationSummary">
    <rdfs:label>ValidationSummary</rdfs:label>
    <rdfs:comment>
      A validation summary provides a succinct description of the result of a validation process. It reports the
      validity of the document instance with respect to a schema and all validation results.
    </rdfs:comment>
    <rdf:type rdf:resource="http://www.w3.org/ns/shacl#NodeShape"/>
    <sh:property>
      <sh:PropertyShape>
        <sh:path rdf:resource="#isValid"/>
        <sh:datatype rdf:resource="http://www.w3.org/2001/XMLSchema#boolean"/>
        <sh:maxCount rdf:datatype="http://www.w3.org/2001/XMLSchema#integer">1</sh:maxCount>
      </sh:PropertyShape>
    </sh:property>
    <sh:property>
      <sh:PropertyShape>
        <sh:path rdf:resource="#result"/>
        <sh:nodeKind rdf:resource="http://www.w3.org/ns/shacl#BlankNode"/>
        <sh:class rdf:resource="#ValidationResult"/>
      </sh:PropertyShape>
    </sh:property>
  </rdfs:Class>

  <rdfs:Class rdf:about="#LineColumnLocator">
    <rdfs:label>LineColumnLocator</rdfs:label>
    <rdfs:comment>Describes a location through line and column number.</rdfs:comment>
    <rdfs:subClassOf rdf:resource="#Locator"/>
    <rdf:type rdf:resource="http://www.w3.org/ns/shacl#NodeShape"/>
    <sh:property>
      <sh:PropertyShape>
        <sh:path rdf:resource="#line"/>
        <sh:datatype rdf:resource="http://www.w3.org/2001/XMLSchema#int"/>
        <sh:maxCount rdf:datatype="http://www.w3.org/2001/XMLSchema#int">1</sh:maxCount>
        <sh:minCount rdf:datatype="http://www.w3.org/2001/XMLSchema#int">1</sh:minCount>
      </sh:PropertyShape>
    </sh:property>
    <sh:property>
      <sh:PropertyShape>
        <sh:path rdf:resource="#column"/>
        <sh:datatype rdf:resource="http://www.w3.org/2001/XMLSchema#int"/>
        <sh:maxCount rdf:datatype="http://www.w3.org/2001/XMLSchema#int">1</sh:maxCount>
        <sh:minCount rdf:datatype="http://www.w3.org/2001/XMLSchema#int">1</sh:minCount>
      </sh:PropertyShape>
    </sh:property>
  </rdfs:Class>

  <rdfs:Class rdf:about="#Locator">
    <rdfs:label>Locator</rdfs:label>
    <rdfs:comment>Describes the location of an information item in a document.</rdfs:comment>
    <rdf:type rdf:resource="http://www.w3.org/ns/shacl#NodeShape"/>
  </rdfs:Class>

  <rdfs:Class rdf:about="#XPathLocator">
    <rdfs:label>XPathLocator</rdfs:label>
    <rdfs:comment>Describes a location through an XPath expression.</rdfs:comment>
    <rdfs:subClassOf rdf:resource="#Locator"/>
    <rdf:type rdf:resource="http://www.w3.org/ns/shacl#NodeShape"/>
    <sh:property>
      <sh:PropertyShape>
        <sh:path rdf:resource="#value"/>
        <sh:minCount rdf:datatype="http://www.w3.org/2001/XMLSchema#integer">1</sh:minCount>
        <sh:maxCount rdf:datatype="http://www.w3.org/2001/XMLSchema#integer">1</sh:maxCount>
      </sh:PropertyShape>
    </sh:property>
    <sh:property>
      <sh:PropertyShape>
        <sh:path rdf:resource="#document"/>
        <sh:datatype rdf:resource="http://www.w3.org/2001/XMLSchema#anyURI"/>
        <sh:maxCount rdf:datatype="http://www.w3.org/2001/XMLSchema#integer">1</sh:maxCount>
      </sh:PropertyShape>
    </sh:property>
  </rdfs:Class>

  <rdfs:Class rdf:about="#CustomLocator">
    <rdfs:label>CustomLocator</rdfs:label>
    <rdfs:comment>Describes a location through an implementation defined expression.</rdfs:comment>
    <rdfs:subClassOf rdf:resource="#Locator"/>
    <rdf:type rdf:resource="http://www.w3.org/ns/shacl#NodeShape"/>
  </rdfs:Class>

  <rdfs:Class rdf:about="#ValidationResult">
    <rdfs:label>ValidationResult</rdfs:label>
    <rdf:type rdf:resource="http://www.w3.org/ns/shacl#NodeShape"/>
    <sh:property>
      <sh:PropertyShape>
        <sh:path rdf:resource="#message"/>
        <sh:minCount rdf:datatype="http://www.w3.org/2001/XMLSchema#int">1</sh:minCount>
        <sh:nodeKind rdf:resource="http://www.w3.org/ns/shacl#Literal"/>
      </sh:PropertyShape>
    </sh:property>
    <sh:property>
      <sh:PropertyShape>
        <sh:path rdf:resource="#instanceLocation"/>
        <sh:nodeKind rdf:resource="http://www.w3.org/ns/shacl#BlankNode"/>
      </sh:PropertyShape>
    </sh:property>
    <sh:property>
      <sh:PropertyShape>
        <sh:path rdf:resource="#schemaLocation"/>
        <sh:nodeKind rdf:resource="http://www.w3.org/ns/shacl#BlankNode"/>
      </sh:PropertyShape>
    </sh:property>
  </rdfs:Class>

  <rdfs:Property rdf:about="#result">
    <rdfs:label>result</rdfs:label>
    <rdfs:comment>
      Connects a validation summary with a validation result produced by the validation process.
    </rdfs:comment>
    <rdfs:domain rdf:resource="#ValidationSummary"/>
    <rdfs:range rdf:resource="#ValidationResult"/>
  </rdfs:Property>

  <rdfs:Property rdf:about="#instanceLocation">
    <rdfs:label>instanceLocation</rdfs:label>
    <rdfs:comment>Connects a validation result with one or more significant locations in the instance document.</rdfs:comment>
    <rdfs:domain rdf:resource="#ValidationResult"/>
    <rdfs:range rdf:resource="#Locator"/>
  </rdfs:Property>

  <rdfs:Property rdf:about="#isValid">
    <rdfs:label>isValid</rdfs:label>
    <rdfs:comment>The object of the predicate is a xsd:boolean that denotes the result of the validation.</rdfs:comment>
    <rdfs:domain rdf:resource="#ValidationSummary"/>
    <rdfs:range rdf:resource="http://www.w3.org/2001/XMLSchema#boolean"/>
  </rdfs:Property>

  <rdfs:Property rdf:about="#message">
    <rdfs:label>message</rdfs:label>
    <rdfs:comment>A human readable description of a validation result.</rdfs:comment>
    <rdfs:domain rdf:resource="#ValidationResult"/>
    <rdfs:range rdf:resource="http://www.w3.org/1999/02/22-rdf-syntax-ns#langString"/>
  </rdfs:Property>

  <rdfs:Property rdf:about="#schemaLocation">
    <rdfs:label>schemaLocation</rdfs:label>
    <rdfs:comment>Connects a validation result with one or more significant locations in the schema document.</rdfs:comment>
    <rdfs:domain rdf:resource="#ValidationResult"/>
    <rdfs:range rdf:resource="#Locator"/>
  </rdfs:Property>

  <rdfs:Property rdf:about="#value">
    <rdfs:label>value</rdfs:label>
  </rdfs:Property>

  <rdfs:Property rdf:about="#document">
    <rdfs:label>document</rdfs:label>
    <rdfs:range rdf:resource="http://www.w3.org/2001/XMLSchema#anyURI"/>
    <rdfs:domain rdf:resource="#Locator"/>
  </rdfs:Property>

  <rdfs:Property rdf:about="#column">
    <rdfs:label>column</rdfs:label>
    <rdfs:domain rdf:resource="#LineColumnLocator"/>
    <rdfs:range rdf:resource="http://www.w3.org/2001/XMLSchema#integer"/>
  </rdfs:Property>

  <rdfs:Property rdf:about="#line">
    <rdfs:label>line</rdfs:label>
    <rdfs:domain rdf:resource="#LineColumnLocator"/>
    <rdfs:range rdf:resource="http://www.w3.org/2001/XMLSchema#integer"/>
  </rdfs:Property>

</rdf:RDF>
